\section{Appendix: Continuation of Analytical Solutions}\label{appendix-b}\thispagestyle{SectionFirstPage} % Hide headers on the first page of the section
\setcounter{figure}{0}
\setcounter{table}{0}
Recall that by transforming the ODE we obtained the form
\begin{equation} \label{eq:first}
	z^{\prime\prime} = x_{0} \beta z^{\prime} e^{-\frac{\beta z}{\gamma}} - \gamma z^{\prime}
\end{equation}
From here we need to introduce a new function 
\begin{equation} \label{eq:second}
	u = e^{-\frac{\beta}{\gamma}z}, \quad u_0 = e^{-\frac{\beta}{\gamma}N_3}\\
\end{equation}
Also note that we got the initial value by substituting $z$ with $z(0)$.\\
Next we substitute (\ref{eq:second}) into (\ref{eq:first}) and by doing a lot of simplification we get
\begin{equation} \label{eq:third}
	u(u)^{\prime\prime} - (u^{\prime})^2 + (\gamma - x_0\beta u)u(u)^\prime = 0
\end{equation}
Now we introduce another function $\phi = t^{\prime}_{u}$, and by substituting it back we get
\begin{equation} \label{eq:forth}
	\phi^{\prime}_u + \phi\frac{1}{u} = (\gamma-x_0\beta u)\phi^2
\end{equation}
which is a Bernoulli type differential equation with the solution given as
\begin{equation} \label{eq:fifth}
	\phi = \frac{1}{u(C_1-\gamma \ln u + x_0\beta u)}
\end{equation}
where $C_1$ is an integration constant. Since $\phi = t^{\prime}_{u}$ by integrating (\ref{eq:fifth}) we get an equation for time
\begin{equation} \label{eq:sixth}
	t = \int_{u_0}^{u} \frac{du}{u(C_1-\gamma \ln u + x_0\beta u)}
\end{equation}
hence with all of this we can get the parametric equation for the simple SIR model with $u$ taken as parameter
\begin{align*} \label{eq:parameter}
	x &= x_0u,\\
	y &= \frac{\gamma}{\beta}\ln u - x_0u - \frac{C_1}{\beta},\\
	z &= -\frac{\gamma}{\beta}\ln u
\end{align*}
and by adding them we can obtain than $C_1 = -\beta N$.
